src/Ex/Mesi/MesiInvB.v
@@ -15,6 +15,57 @@ Local Open Scope list.
 Local Open Scope hvec.
 Local Open Scope fmap.
 
+(** Move to [TopoTemplate.v] *)
+Lemma tree2Topo_root_not_in_tl_li:
+  forall tr (Htr: tr <> Node nil) bidx,
+    ~ In (rootOf (fst (tree2Topo tr bidx))) (tl (c_li_indices (snd (tree2Topo tr bidx)))).
+Proof.
+  intros.
+  pose proof (tree2Topo_WfCIfc tr bidx).
+  destruct H as [? _].
+  rewrite c_li_indices_head_rootOf in H by assumption.
+  inv H.
+  intro Hx; elim H2.
+  apply in_or_app; left; assumption.
+Qed.
+
+Lemma tree2Topo_root_not_in_l1:
+  forall tr (Htr: tr <> Node nil) bidx,
+    ~ In (rootOf (fst (tree2Topo tr bidx))) (c_l1_indices (snd (tree2Topo tr bidx))).
+Proof.
+  intros.
+  pose proof (tree2Topo_WfCIfc tr bidx).
+  destruct H as [? _].
+  rewrite c_li_indices_head_rootOf in H by assumption.
+  inv H.
+  intro Hx; elim H2.
+  apply in_or_app; right; assumption.
+Qed.
+
+Lemma tree2Topo_root_not_l1ExtOf:
+  forall tr (Htr: tr <> Node nil) bidx oidx,
+    In oidx (c_l1_indices (snd (tree2Topo tr bidx))) ->
+    l1ExtOf oidx <> rootOf (fst (tree2Topo tr bidx)).
+Proof.
+  intros.
+  assert (In (rqUpFrom (l1ExtOf oidx)) (c_merqs (snd (tree2Topo tr bidx)))).
+  { rewrite c_merqs_l1_rqUpFrom.
+    apply in_map_iff.
+    eexists; repeat split.
+    assumption.
+  }
+  assert (In (rqUpFrom (rootOf (fst (tree2Topo tr bidx))))
+             (c_minds (snd (tree2Topo tr bidx)))).
+  { eapply tree2Topo_obj_chns_minds_SubList.
+    { rewrite c_li_indices_head_rootOf by assumption.
+      left; reflexivity.
+    }
+    { simpl; tauto. }
+  }
+  intro Hx; rewrite Hx in H0.
+  eapply DisjList_In_1; [apply tree2Topo_minds_merqs_disj| |]; eauto.
+Qed.
+
 Existing Instance Mesi.ImplOStateIfc.
 
 Section Footprints.
@@ -42,6 +93,21 @@ Section Footprints.
 
 End Footprints.
 
+Section FootprintsOk.
+  Variable (tr: tree).
+  Hypothesis (Htr: tr <> Node nil).
+
+  Let topo: DTree := fst (tree2Topo tr 0).
+  Let cifc: CIfc := snd (tree2Topo tr 0).
+  Let impl: System := impl Htr.
+
+  Theorem mesi_footprints_ok:
+    InvReachable impl step_m (MesiFootprintsInv topo).
+  Proof.
+  Admitted.
+
+End FootprintsOk.
+
 Ltac exfalso_downlock_from oidx Hinv :=
   specialize (Hinv oidx); simpl in Hinv;
   disc_rule_conds_ex;
@@ -54,4 +120,230 @@ Ltac exfalso_downlock_from oidx Hinv :=
     | [Hdfp: DownLockFromParent _ _ |- _] =>
       red in Hdfp; dest; disc_rule_conds_ex; solve_midx_false
     end.
+
+Section InvProof.
+  Variable (tr: tree).
+  Hypothesis (Htr: tr <> Node nil).
+
+  Let topo: DTree := fst (tree2Topo tr 0).
+  Let cifc: CIfc := snd (tree2Topo tr 0).
+  Let impl: System := impl Htr.
+
+  Lemma mesi_RootChnInv_init:
+    Invariant.InvInit impl (RootChnInv tr 0).
+  Proof.
+    do 2 (red; simpl).
+    intros.
+    intro Hx; do 2 (red in Hx).
+    dest_in.
+  Qed.
+
+  Ltac disc_RootChnInv :=
+    intros;
+    let Hx := fresh "H" in
+    intro Hx;
+    repeat
+      match goal with
+      | [H: In _ (subtreeChildrenIndsOf _ _) |- _] =>
+        apply subtreeChildrenIndsOf_parentIdxOf in H; auto
+      | [Hm: InMPI (enqMsgs _ _) _ |- _] =>
+        apply InMP_enqMsgs_or in Hm; destruct Hm
+      | [Hinv: _ -> _ -> ~ InMPI _ _,  Hm: InMP _ _ (deqMsgs _ _) |- _] =>
+        apply InMP_deqMsgs in Hm; eapply Hinv; eauto
+      | [H: In (idOf ?idm, valOf ?idm) _ |- _] =>
+        let midx := fresh "midx" in
+        let msg := fresh "msg" in
+        destruct idm as [midx msg]; simpl in *
+      end;
+    disc_rule_conds_ex.
+
+  Ltac solve_RootChnInv :=
+    repeat
+      match goal with
+      | [H1: In _ ?l, H2: SubList ?l (subtreeChildrenIndsOf _ _) |- _] =>
+        apply H2 in H1
+      | [H: In _ (subtreeChildrenIndsOf _ _) |- _] =>
+        apply subtreeChildrenIndsOf_parentIdxOf in H; auto
+      | [H: In _ (map _ _) |- _] => apply in_map_iff in H; dest
+      | [H: (_, _) = (_, _) |- _] => inv H
+      | [H: _ \/ _ \/ _ |- _] => destruct H as [|[|]]; try discriminate
+      | [H: rqUpFrom _ = rqUpFrom _ |- _] => inv H
+      | [H: rsUpFrom _ = rsUpFrom _ |- _] => inv H
+      | [H: downTo _ = downTo _ |- _] => inv H
+
+      | [H: parentIdxOf _ ?oidx = Some ?oidx |- _] =>
+        exfalso; eapply parentIdxOf_not_eq; eauto
+      | [H1: ?oidx = rootOf _, H2: parentIdxOf _ ?oidx = Some _ |- _] => rewrite H1 in H2
+      | [H: parentIdxOf _ (rootOf _) = Some _ |- _] =>
+        eapply parentIdxOf_child_not_root; eauto
+      | [H: In (rootOf _) (tl (c_li_indices _)) |- _] =>
+        exfalso; eapply tree2Topo_root_not_in_tl_li; eauto
+      | [H: In (rootOf _) (c_l1_indices _) |- _] =>
+        exfalso; eapply tree2Topo_root_not_in_l1; eauto
+      | [H1: In ?oidx (c_l1_indices _), H2: l1ExtOf ?oidx = rootOf _ |- _] =>
+        eapply tree2Topo_root_not_l1ExtOf; eauto
+      end.
+
+  Lemma mesi_RootChnInv_step:
+    Invariant.InvStep impl step_m (RootChnInv tr 0).
+  Proof.
+    red; intros.
+    pose proof (tree2Topo_TreeTopoNode tr 0) as Htn.
+    pose proof (footprints_ok
+                  (mesi_GoodORqsInit Htr)
+                  (mesi_GoodRqRsSys Htr) H) as Hftinv.
+    pose proof (mesi_footprints_ok H) as Hmftinv.
+    inv H1; [assumption|..].
+
+    1: {
+      red; simpl; intros.
+      intro Hx; apply InMP_enqMsgs_or in Hx.
+      destruct Hx; [|eapply H0; eauto].
+      apply in_map with (f:= idOf) in H4; simpl in H4.
+      apply H3 in H4; simpl in H4.
+      eapply DisjList_In_1.
+      + apply tree2Topo_minds_merqs_disj.
+      + eassumption.
+      + eapply tree2Topo_obj_chns_minds_SubList.
+        * rewrite c_li_indices_head_rootOf by assumption.
+          left; reflexivity.
+        * destruct H1 as [|[|]]; rewrite H1; simpl; tauto.
+    }
+
+    1: {
+      red; simpl; intros.
+      intro Hx; apply InMP_deqMsgs in Hx.
+      eapply H0; eauto.
+    }
+
+    simpl in H2; destruct H2; [subst|apply in_app_or in H1; destruct H1].
+
+    - (*! Cases for the main memory *)
+
+      (** Abstract the root. *)
+      unfold RootChnInv in *; simpl in *.
+      remember (rootOf (fst (tree2Topo tr 0))) as oidx; clear Heqoidx.
+
+      (** Do case analysis per a rule. *)
+      apply in_app_or in H3; destruct H3.
+
+      1: { (** Rules per a child *)
+        apply concat_In in H1; destruct H1 as [crls [? ?]].
+        apply in_map_iff in H1; destruct H1 as [cidx [? ?]]; subst.
+        dest_in; try (disc_RootChnInv; solve_RootChnInv; fail).
+      }
+
+      dest_in.
+      { disc_RootChnInv.
+        red in Hmftinv; simpl in Hmftinv.
+        specialize (Hmftinv oidx).
+        disc_rule_conds_ex.
+        rewrite H4 in Hmftinv.
+        simpl in Hmftinv; destruct Hmftinv as [cidx [? ?]].
+        rewrite Hidx in H7; inv H7.
+        solve_RootChnInv.
+      }
+      { disc_RootChnInv.
+        move Hmftinv at bottom.
+        red in Hmftinv; simpl in Hmftinv.
+        specialize (Hmftinv oidx).
+        disc_rule_conds_ex.
+        rewrite H9 in Hmftinv.
+        simpl in Hmftinv; destruct Hmftinv as [cidx [? ?]].
+        rewrite Hidx in H10; inv H10.
+        solve_RootChnInv.
+      }
+
+    - (*! Cases for Li caches *)
+      unfold RootChnInv in *; simpl in *.
+
+      (** Do case analysis per a rule. *)
+      apply in_map_iff in H1; destruct H1 as [oidx [? ?]]; subst; simpl in *.
+      apply in_app_or in H3; destruct H3.
+
+      1: { (** Rules per a child *)
+        apply concat_In in H1; destruct H1 as [crls [? ?]].
+        apply in_map_iff in H1; destruct H1 as [cidx [? ?]]; subst.
+        dest_in; abstract (disc_RootChnInv; solve_RootChnInv; fail).
+      }
+
+      dest_in.
+      all: try (disc_RootChnInv; solve_RootChnInv; fail).
+      all: try (disc_RootChnInv;
+                derive_footprint_info_basis oidx;
+                derive_child_chns cidx;
+                disc_rule_conds_ex;
+                solve_RootChnInv;
+                fail).
+      all: try (disc_RootChnInv;
+                derive_footprint_info_basis oidx;
+                [|exfalso_downlock_from oidx Hmftinv;
+                  derive_child_chns x;
+                  solve_midx_false];
+                derive_child_chns upCIdx;
+                disc_rule_conds_ex;
+                solve_RootChnInv;
+                fail).
+
+      { disc_RootChnInv.
+        derive_footprint_info_basis oidx.
+        1: {
+          exfalso_downlock_from oidx Hmftinv.
+          derive_child_chns (obj_idx upCObj).
+          disc_rule_conds_ex.
+        }
+        eapply edgeDownTo_Some in H10; eauto; dest.
+        derive_child_chns oidx.
+        disc_rule_conds_ex.
+        solve_RootChnInv.
+      }
+      { disc_RootChnInv.
+        derive_footprint_info_basis oidx.
+        1: {
+          exfalso_downlock_from oidx Hmftinv.
+          derive_child_chns (obj_idx upCObj).
+          disc_rule_conds_ex.
+        }
+        eapply edgeDownTo_Some in H17; eauto; dest.
+        derive_child_chns oidx.
+        disc_rule_conds_ex.
+        solve_RootChnInv.
+      }
+
+    - (*! Cases for L1 caches *)
+      unfold RootChnInv in *; simpl in *.
+
+      (** Do case analysis per a rule. *)
+      apply in_map_iff in H1; destruct H1 as [oidx [? ?]]; subst.
+      dest_in; try (disc_RootChnInv; solve_RootChnInv; fail).
+
+      + disc_RootChnInv.
+        derive_footprint_info_basis oidx.
+        derive_child_chns cidx.
+        disc_rule_conds_ex.
+        solve_RootChnInv.
+      + disc_RootChnInv.
+        derive_footprint_info_basis oidx.
+        derive_child_chns cidx.
+        disc_rule_conds_ex.
+        solve_RootChnInv.
+      + disc_RootChnInv.
+        derive_footprint_info_basis oidx.
+        derive_child_chns cidx.
+        disc_rule_conds_ex.
+        solve_RootChnInv.
+
+        Unshelve.
+        all: assumption.
+  Qed.
+
+  Theorem mesi_RootChnInv_ok:
+    InvReachable impl step_m (RootChnInv tr 0).
+  Proof.
+    apply inv_reachable.
+    - apply mesi_RootChnInv_init.
+    - apply mesi_RootChnInv_step.
+  Qed.
+  
+End InvProof.
 
