src/Ex/Template.v
@@ -2,4 +2,4 @@ Require Import List FMap Omega.
 Require Import Common Topology Syntax IndexSupport.
 Require Import RqRsLang.
 
-Require Export Ex.TopoTemplate Ex.RuleTemplate.
+Require Export Ex.TopoTemplate Ex.RuleTemplate Ex.InvTemplate Ex.SimTemplate.
